src/Implementations/Transaction/Transaction.v
@@ -12,22 +12,22 @@ Fixpoint get_latest (txn: list (addr * value)) a :=
   end.
 
 Definition start :=
-  _ <- |TCCO| Put [];
+  _ <- |TCCO| Delete _;
   Ret tt.
 
 (** Reverses before submitting **)
 Definition commit :=
   txn <- |TCCO| Get _;
-  let al := fst (split (rev txn)) in
-  let vl := snd (split (rev txn)) in
+  let al := map fst (rev txn) in
+  let vl := map snd (rev txn) in
   let dedup_al := dedup_last addr_dec al in
   let dedup_vl := dedup_by_list addr_dec al vl in
   _ <- |TCDO| Write dedup_al dedup_vl;
-  _ <- |TCCO| Put [];
+  _ <- |TCCO| Delete _;
   Ret tt.
 
 Definition abort :=
-  _ <- |TCCO| Put [];
+  _ <- |TCCO| Delete _;
   Ret tt.
 
 (* if you read out of bounds, you get 0 block *)
@@ -49,7 +49,7 @@ Definition write a v :=
   if lt_dec a data_length then
     txn <- |TCCO| Get _;
     if lt_dec (length txn) log_length then
-      _ <- |TCCO| Put ((a, v)::txn);
+      _ <- |TCCO| Put (a, v);
       Ret tt
     else
       Ret tt
@@ -59,3 +59,12 @@ Definition write a v :=
 Definition recover :=
   _ <- |TCDO| Recover;
   Ret tt.
+
+Definition transaction_rep (tcd: TransactionCacheLang.(state)) (td: (@mem addr addr_dec value) * (@total_mem addr addr_dec value)):=
+  let al := map fst (fst tcd) in
+  let vl := map snd (fst tcd) in
+  let dedup_al := dedup_last addr_dec al in
+  let dedup_vl := dedup_by_list addr_dec al vl in
+  fst td = Mem.upd_batch empty_mem dedup_al dedup_vl /\
+  snd td = snd tcd.
+  
