src/Layers/AbstractLayers/TransactionalDisk/TransactionalDiskLayer.v
@@ -3,8 +3,14 @@ Import ListNotations.
 
 Set Implicit Arguments.
 
-Section TransactionalDisk.
+Definition apply_mem {A AEQ V} (m: @mem A AEQ V) (tm: @total_mem A AEQ V):=
+  fun a => match m a with
+        | Some v => v
+        | None => tm a
+        end.
 
+Section TransactionalDisk.
+  
   Variable disk_size: nat.
 
   Inductive token' :=
@@ -14,7 +20,7 @@ Section TransactionalDisk.
   | Cont : token'
   | TxnFull : token'.
 
-  Definition state' := ((disk value) * (disk value))%type.
+  Definition state' := ((@mem addr addr_dec value) * (@total_mem addr addr_dec value))%type.
   
   Inductive transactional_disk_prog : Type -> Type :=
   | Start : transactional_disk_prog unit
@@ -23,461 +29,92 @@ Section TransactionalDisk.
   | Commit : transactional_disk_prog unit
   | Abort : transactional_disk_prog unit
   | Recover : transactional_disk_prog unit.
-   
+
   Inductive exec' :
-    forall T, token' ->  state' -> transactional_disk_prog T -> @Result state' T -> Prop :=
+    forall T, user -> token' ->  state' -> transactional_disk_prog T -> @Result state' T -> Prop :=
   | ExecStart : 
-      forall s,
+      forall s u,
         let c := fst s in
         let d := snd s in
-        exec' Cont s Start (Finished (empty_mem, d) tt)
+        exec' u Cont s Start (Finished (empty_mem, d) tt)
               
   | ExecReadInbound : 
-      forall s a v,
+      forall s a v u,
         let c := fst s in
         let d := snd s in
         a < disk_size ->
         (c a = Some v \/
-        (c a = None /\ d a = Some v)) ->
-        exec' Cont s (Read a) (Finished s v)
+        (c a = None /\ d a = v)) ->
+        exec' u Cont s (Read a) (Finished s v)
 
   | ExecReadOutbound : 
-      forall s a,
+      forall s a u,
         a >= disk_size ->
-        exec' Cont s (Read a) (Finished s value0)
+        exec' u Cont s (Read a) (Finished s value0)
              
   | ExecWriteInbound :
-      forall s a v,
+      forall s a v u,
         let c := fst s in
         let d := snd s in
         a < disk_size ->
-        d a <> None ->
-        exec' Cont s (Write a v) (Finished ((upd c a v), d) tt)
+        exec' u Cont s (Write a v) (Finished ((Mem.upd c a v), d) tt)
 
   | ExecWriteInboundFull :
-      forall s a v,
+      forall s a v u,
         let c := fst s in
         let d := snd s in
         a < disk_size ->
-        d a <> None ->
-        exec' TxnFull s (Write a v) (Finished s tt)
+        exec' u TxnFull s (Write a v) (Finished s tt)
               
   | ExecWriteOutbound :
-      forall s a v,
+      forall s a v u,
         a >= disk_size ->
-        exec' Cont s (Write a v) (Finished s tt)
+        exec' u Cont s (Write a v) (Finished s tt)
 
   | ExecCommit : 
-      forall s,
+      forall s u,
         let c := fst s in
         let d := snd s in
-        exec' Cont s Commit (Finished (empty_mem, mem_union c d) tt)
+        exec' u Cont s Commit (Finished (empty_mem, apply_mem c d) tt)
 
   | ExecAbort : 
-      forall s,
+      forall s u,
         let c := fst s in
         let d := snd s in
-        exec' Cont s Abort (Finished (empty_mem, d) tt)
+        exec' u Cont s Abort (Finished (empty_mem, d) tt)
 
   | ExecRecover : 
-      forall s,
-        exec' Cont s Recover (Finished s tt)
+      forall s u,
+        exec' u Cont s Recover (Finished s tt)
 
   | ExecCrashBefore :
-      forall d T (p: transactional_disk_prog T),
-        exec' CrashBefore d p (Crashed d)
+      forall d T (p: transactional_disk_prog T) u,
+        exec' u CrashBefore d p (Crashed d)
 
-  | ExecCrashAfter :
-      forall s s' T (p: transactional_disk_prog T),
-        (exists v, exec' Cont s p (Finished s' v)) ->
-        exec' CrashAfter s p (Crashed s')
+  | ExecCommitCrashAfter :
+      forall s u,
+        let c := fst s in
+        let d := snd s in
+        exec' u CrashAfter s Commit (Crashed (empty_mem, apply_mem c d)).
 
-  | ExecCrashDuringCommit :
-      forall s c d,
-        (exists v, exec' Cont s Commit (Finished (c, d) v)) ->
-        exec' CrashDuringCommit s Commit (Crashed (fst s, d)).
+  (* 
+     | ExecCrashDuringCommit :
+      forall s c d u,
+        (exists v, exec' u Cont s Commit (Finished (c, d) v)) ->
+        exec' u CrashDuringCommit s Commit (Crashed (fst s, d)). *)
 
   Hint Constructors exec' : core.
 
-   Definition weakest_precondition' T (p: transactional_disk_prog T) :=
-   match p in transactional_disk_prog T' return (T' -> state' -> Prop) -> token' -> state' -> Prop with
-   | Start =>
-     (fun Q o s =>
-       let c := fst s in
-       let d := snd s in
-       o = Cont /\
-       Q tt (empty_mem, d))
-   | Read a =>
-     (fun Q o s =>
-        let c := fst s in
-        let d := snd s in
-        (
-          o = Cont /\
-          a < disk_size /\ 
-          exists v,
-            (c a = Some v \/ (c a = None /\ d a = Some v)) /\
-            Q v s
-        ) \/
-        (
-          o = Cont /\
-          a >= disk_size /\
-          Q value0 s
-        )
-     )
-   | Write a v =>
-     (fun Q o s =>
-       let c := fst s in
-       let d := snd s in
-       
-       (
-         o = Cont /\
-         a < disk_size /\
-         d a <> None /\
-         Q tt ((upd c a v), d)
-       ) \/
-       (
-         o = TxnFull /\
-         a < disk_size /\
-         d a <> None /\
-         Q tt s
-       ) \/
-       (
-         o = Cont /\
-         a >= disk_size /\
-         Q tt s
-       )
-     )
-   | Commit =>
-     (fun Q o s =>
-       let c := fst s in
-       let d := snd s in
-       o = Cont /\
-       Q tt (empty_mem, mem_union c d))
-   | Abort =>
-     (fun Q o s =>
-       let c := fst s in
-       let d := snd s in
-       o = Cont /\
-       Q tt (empty_mem, d))
-   | Recover =>
-     (fun Q o s =>
-       o = Cont /\
-       Q tt s)
-   end.
-
-  Definition weakest_crash_precondition' T (p: transactional_disk_prog T) :=
-    match p in transactional_disk_prog T' return (state' -> Prop) -> token' -> state' -> Prop with
-    | Start =>
-      (fun Q o s =>
-         let c := fst s in
-         let d := snd s in
-         (o = CrashBefore /\
-          Q s) \/
-         (o = CrashAfter /\
-          Q (empty_mem, d)))
-   | Read a =>
-     (fun Q o s =>
-        let c := fst s in
-        let d := snd s in
-        (
-          o = CrashBefore /\
-          Q s
-        ) \/
-        (
-          o = CrashAfter /\
-          a < disk_size /\
-          Q s /\
-          exists v,
-            c a = Some v \/
-            (c a = None /\ d a = Some v)
-        ) \/
-        (
-          o = CrashAfter /\
-          a >= disk_size /\
-          Q s
-        )
-     )
-   | Write a v =>
-     (fun Q o s =>
-        let c := fst s in
-        let d := snd s in
-        (
-          o = CrashBefore /\
-          Q s
-        ) \/
-        (
-          o = CrashAfter /\
-          a < disk_size /\
-          d a <> None /\
-          Q (upd c a v, d)
-        ) \/
-        (
-          o = CrashAfter /\
-          a >= disk_size /\
-          Q s
-        )
-     )
-   | Commit =>
-     (fun Q o s =>
-       let c := fst s in
-       let d := snd s in
-       (o = CrashBefore /\
-        Q s) \/
-       (o = CrashDuringCommit /\
-        Q (c, mem_union c d)) \/
-       (o = CrashAfter /\
-        Q (empty_mem, mem_union c d)))
-   | Abort =>
-      (fun Q o s =>
-         let c := fst s in
-         let d := snd s in
-         (o = CrashBefore /\
-          Q s) \/
-         (o = CrashAfter /\
-          Q (empty_mem, d)))
-   | Recover =>
-      (fun Q o s =>
-         (o = CrashBefore /\
-          Q s) \/
-         (o = CrashAfter /\
-          Q s))
-    end.
-
-  Definition strongest_postcondition' T (p: transactional_disk_prog T) :=
-    match p in transactional_disk_prog T' return (token' -> state' -> Prop) -> T' -> state' -> Prop with
-    | Start =>
-      fun P t s' =>
-        exists s,
-         let c := fst s in
-         let d := snd s in
-         P Cont s /\
-         t = tt /\
-         s' = (empty_mem, d)
-   | Read a =>
-     fun P t s' =>
-       exists s,
-         let c := fst s in
-         let d := snd s in
-         (
-           P Cont s /\
-           a < disk_size /\
-           s' = s /\
-           exists v,
-             ( c a = Some v \/ (c a = None /\ d a = Some v) ) /\
-             t = v 
-         ) \/
-         (
-           P Cont s /\
-           s' = s /\
-           a >= disk_size /\
-           t = value0
-         )
-   | Write a v =>
-     fun P t s' =>
-       exists s,
-       let c := fst s in
-       let d := snd s in
-       (
-         P Cont s /\
-         a < disk_size /\
-         t = tt /\
-         d a <> None /\
-         s' = ((upd c a v), d)
-       ) \/
-       (
-         P TxnFull s /\
-         a < disk_size /\
-         d a <> None /\
-         t = tt /\
-         s' = s
-       ) \/
-       (
-         P Cont s /\
-         a >= disk_size /\
-         t = tt /\
-         s' = s
-       )
-         
-   | Commit =>
-      fun P t s' =>
-        exists s,
-         let c := fst s in
-         let d := snd s in
-         P Cont s /\
-         t = tt /\
-         s' = (empty_mem, mem_union c d)
-   | Abort =>
-      fun P t s' =>
-        exists s,
-         let c := fst s in
-         let d := snd s in
-         P Cont s /\
-         t = tt /\
-         s' = (empty_mem, d)
-   | Recover =>
-      fun P t s' =>
-        exists s,
-         P Cont s /\
-         t = tt /\
-         s' = s
-   end.
-
-  Definition strongest_crash_postcondition' T (p: transactional_disk_prog T) :=
-    match p in transactional_disk_prog T' return (token' -> state' -> Prop) -> state' -> Prop with
-    | Start =>
-      fun P s' =>
-        exists s,
-          let c := fst s in
-          let d := snd s in
-          (P CrashBefore s /\
-           s' = s) \/
-          (P CrashAfter s /\
-           s' = (empty_mem, d))
-    | Read a =>
-     fun P s' =>
-       exists s,
-         let c := fst s in
-         let d := snd s in
-         (
-           P CrashBefore s /\
-           s' = s
-         ) \/
-         (
-           P CrashAfter s /\
-           a < disk_size /\
-           s' = s /\
-           (exists v, c a = Some v \/ (c a = None /\ d a = Some v))
-         ) \/
-         (
-           P CrashAfter s /\
-           a >= disk_size /\
-           s' = s
-         )
-           
-   | Write a v =>
-     fun P s' =>
-       exists s,
-         let c := fst s in
-         let d := snd s in
-         (
-           P CrashBefore s /\
-           s' = s
-         ) \/
-         (
-           P CrashAfter s /\
-           a < disk_size /\
-           d a <> None /\
-           s' = (upd c a v, d)
-         ) \/
-         (
-           P CrashAfter s /\
-           a >= disk_size /\
-           s' = s
-         )
-           
-   | Commit =>
-      fun P s' =>
-       exists s,
-         let c := fst s in
-         let d := snd s in
-         (P CrashBefore s /\
-          s' = s) \/
-         (P CrashAfter s /\
-          s' = (empty_mem, mem_union c d)) \/
-         (P CrashDuringCommit s /\
-          s' = (fst s, mem_union c d))
-   | Abort =>
-      fun P s' =>
-        exists s,
-          let c := fst s in
-          let d := snd s in
-          (P CrashBefore s /\
-           s' = s) \/
-          (P CrashAfter s /\
-           s' = (empty_mem, d))
-    | Recover =>
-      fun P s' =>
-        exists s,
-          (P CrashBefore s /\
-           s' = s) \/
-          (P CrashAfter s /\
-           s' = s)
-    end.
-  
-  Theorem sp_complete':
-    forall T (p: transactional_disk_prog T) P (Q: _ -> _ -> Prop),
-      (forall t s', strongest_postcondition' p P t s' -> Q t s') <->
-      (forall o s s' t, P o s -> exec' o s p (Finished s' t) -> Q t s').
-  Proof.
-    intros; destruct p; simpl; eauto;
-    split; intros;
-    try match goal with
-        | [H: exec' _ _ _ _ |- _] =>
-          inversion H; clear H
-        end; cleanup;
-    try solve [ eapply H; eauto;
-    try solve [ repeat (eexists; intuition eauto) ];
-    try solve [ eexists; intuition eauto; eexists; intuition eauto ] ];
-    repeat split_ors; cleanup; eauto.
-  Qed.
-
-  Theorem scp_complete':
-    forall T (p: transactional_disk_prog T) P (Q:  _ -> Prop),
-      (forall s', strongest_crash_postcondition' p P s' -> Q s') <->
-      (forall o s s', P o s -> exec' o s p (Crashed s') -> Q s').
-  Proof.
-    intros; destruct p; simpl; eauto;
-    split; intros; cleanup;
-    repeat (try split_ors; try inversion H1; clear H1; cleanup; eauto);
-    try split_ors; cleanup;
-    try solve [ eapply H; eauto;
-    try solve [ eexists; right; intuition eauto];    
-    try solve [ split_ors; cleanup; econstructor; eauto ] ];
-    repeat split_ors; cleanup; eauto.
-  Qed.
-
-  Theorem wp_complete':
-    forall T (p: transactional_disk_prog T) H Q,
-      (forall o s, H o s -> weakest_precondition' p Q o s) <->
-      (forall o s, H o s -> (exists s' v, exec' o s p (Finished s' v) /\ Q v s')).
-  Proof.
-    intros; destruct p; simpl; eauto;
-    split; intros;
-    specialize H0 with (1:= X);
-    cleanup; eauto;
-    try inversion H0; cleanup; eauto.
-    intuition eauto.
-    repeat (split_ors; cleanup);
-    do 2 eexists; eauto.
-    right; eauto.
-  Qed.
-  
-  Theorem wcp_complete':
-    forall T (p: transactional_disk_prog T) H C,
-      (forall o s, H o s -> weakest_crash_precondition' p C o s) <->
-      (forall o s, H o s -> (exists s', exec' o s p (Crashed s') /\ C s')).
-  Proof.
-    unfold weakest_crash_precondition';
-    intros; destruct p; simpl; eauto;
-    split; intros; cleanup;
-    specialize H0 with (1:= X);
-    try split_ors; cleanup; repeat (try inversion H0; try clear H0; cleanup; eauto);
-    try solve [eexists; econstructor; eauto].
-    right; intuition eauto.
-    right; intuition eauto.
-    eexists; split; eauto; econstructor; eauto.
-  Qed.
-
   Theorem exec_deterministic_wrt_token' :
-    forall o s T (p: transactional_disk_prog T) ret1 ret2,
-      exec' o s p ret1 ->
-      exec' o s p ret2 ->
+    forall u o s T (p: transactional_disk_prog T) ret1 ret2,
+      exec' u o s p ret1 ->
+      exec' u o s p ret2 ->
       ret1 = ret2.
   Proof.
     intros; destruct p; simpl in *; cleanup;
     repeat
       match goal with
-      | [H: exec' _ _ _ _ |- _] =>
+      | [H: exec' _ _ _ _ _ |- _] =>
         inversion H; clear H; cleanup
       end; eauto;
     repeat split_ors; cleanup; eauto; lia.
@@ -487,22 +124,8 @@ Section TransactionalDisk.
     Build_Core
       transactional_disk_prog
       exec'
-      (*
-        weakest_precondition'
-      weakest_crash_precondition'
-      strongest_postcondition'
-      strongest_crash_postcondition'
-      wp_complete'
-      wcp_complete'
-      sp_complete'
-      scp_complete'
-       *)
       exec_deterministic_wrt_token'.
 
   Definition TransactionalDiskLang := Build_Language TransactionalDiskOperation.
 
 End TransactionalDisk.
-
-Notation "| p |" := (Op (TransactionalDiskOperation _) p)(at level 60).
-Notation "x <-| p1 ; p2" := (Bind (Op (TransactionalDiskOperation _) p1) (fun x => p2))(right associativity, at level 60). 
-Notation "p >> s" := (p s) (right associativity, at level 60, only parsing).
