src/Refinements/TransactionToTransactionalDisk/Definitions.v
@@ -1,129 +1,137 @@
-Require Import Framework FSParameters.
+Require Import Framework FSParameters TotalMem.
 Require Import TransactionCacheLayer TransactionalDiskLayer Transaction.
 Close Scope predicate_scope.
 Import ListNotations.
 
-Local Definition low_op := TransactionCacheOperation.
-Local Definition high_op := (TransactionalDiskOperation data_length).
-Local Definition low := TransactionCacheLang.
-Local Definition high := (TransactionalDiskLang data_length).
+Local Definition imp_op := TransactionCacheOperation.
+Local Definition abs_op := (TransactionalDiskOperation data_length).
+Local Definition imp := TransactionCacheLang.
+Local Definition abs := (TransactionalDiskLang data_length).
 
-Fixpoint apply_list {A AEQ V} (m: @mem A AEQ V) l :=
-  match l with
-  | nil =>
-    m
-  | av :: l' =>
-    apply_list (upd m (fst av) (snd av)) l'
-  end.
-
-Definition compile  T (p2: Operation.prog high_op T) : prog low T.
+Definition compile  T (p2: abs_op.(operation) T) : prog imp T.
   destruct p2.
   exact start.
   exact (read a).
   exact (write a v).
   exact commit.
   exact abort.
+  exact recover.
 Defined.
 
-Definition oracle_refines_to T (d1: state low) (p: Operation.prog high_op T) o1 o2 : Prop :=
+Definition token_refines_to  T u (d1: state imp) (p: Core.operation abs_op T) (get_reboot_state: imp.(state) -> imp.(state)) o1 o2 : Prop :=
      match p with
      | Start =>
        (exists d1' r,
-          exec low o1 d1 start (Finished d1' r) /\
-          o2 = [Cont] /\
-          d1' = (Some [], snd d1)) \/
+          exec imp u o1 d1 start (Finished d1' r) /\
+          o2 = Cont /\
+          d1' = ([], snd d1)) \/
        
        (exists d1',
-          exec low o1 d1 start (Crashed d1') /\
-          ((o2 = [CrashBefore] /\
-            d1' = d1) \/
-           
-           (o2 = [CrashAfter] /\
-            d1' = (Some [], snd d1))))
+          exec imp u o1 d1 start (Crashed d1') /\
+          o2 = CrashBefore /\
+          d1' = d1)
          
      | Read a =>
        (exists d1' r,
-          exec low o1 d1 (read a) (Finished d1' r) /\
-          o2 = [Cont] /\
+          exec imp u o1 d1 (read a) (Finished d1' r) /\
+          o2 = Cont /\
           d1' = d1) \/
        
        (exists d1',
-          exec low o1 d1 (read a) (Crashed d1') /\
-          (o2 = [CrashBefore] \/
-          (o2 = [CrashAfter] /\
-           exists l, fst d1 = Some l /\
-           exists v, get_latest l a = Some v \/ (get_latest l a = None /\ (snd d1) a = Some v))) /\
+          exec imp u o1 d1 (read a) (Crashed d1') /\
+          o2 = CrashBefore /\
           d1' = d1)
          
      | Write a v =>
        (exists d1' r,
-          exec low o1 d1 (write a v) (Finished d1' r) /\          
-          ((o2 = [Cont] /\
+          exec imp u o1 d1 (write a v) (Finished d1' r) /\          
+          ((o2 = Cont /\
             a < data_length /\
-            fst d1 <> None /\
-            d1' = (option_map (fun l => (a, v)::l) (fst d1), snd d1)) \/
-           (o2 = [Cont] /\
+            d1' = ((a, v)::fst d1, snd d1)) \/
+
+           (o2 = Cont /\
             a >= data_length /\
             d1' = d1) \/
-           (exists l,
-              o2 = [TxnFull] /\
-              fst d1 = Some l /\
-              a < data_length /\
-              length l >= log_length /\
-              d1' = d1)
+
+           (o2 = TxnFull /\
+            a < data_length /\
+            length (fst d1) >= log_length /\
+            d1' = d1)
           )
        ) \/
        
        (exists d1',
-          exec low o1 d1 (write a v) (Crashed d1') /\
-          ((o2 = [CrashBefore] /\
-            d1' = d1) \/
-           
-           (o2 = [CrashAfter] /\
-            fst d1 <> None /\
-            d1' = (option_map (fun l => (a, v)::l) (fst d1), snd d1))))
+          exec imp u o1 d1 (write a v) (Crashed d1') /\
+          o2 = CrashBefore /\
+          d1' = d1)
 
      | Commit =>
        (exists d1' r,
-          exec low o1 d1 commit (Finished d1' r) /\
-          o2 = [Cont] /\
-          (exists l, fst d1 = Some l /\
-                d1' = (Some [], mem_union (apply_list empty_mem (rev l)) (snd d1)))) \/
+          exec imp u o1 d1 commit (Finished d1' r) /\
+          o2 = Cont /\
+          d1' = ([], upd_batch (snd d1) (map fst (fst d1)) (map snd (fst d1)))) \/
        
        (exists d1',
-          exec low o1 d1 commit (Crashed d1') /\
-          ((o2 =[CrashBefore] /\
+          exec imp u o1 d1 commit (Crashed d1') /\
+          ((o2 = CrashBefore /\
             d1' = d1) \/
-            (o2 = [CrashDuringCommit] /\
-            (exists l, fst d1 = Some l /\
-                d1' = (Some l,  mem_union (apply_list empty_mem (rev l)) (snd d1) ))) \/
-           (o2 = [CrashAfter] /\
-            (exists l, fst d1 = Some l /\
-                d1' = (Some [],  mem_union (apply_list empty_mem (rev l)) (snd d1) )))))
-         
+           (o2 = CrashAfter /\
+            d1' = ([], upd_batch (snd d1) (map fst (fst d1)) (map snd (fst d1))))))
+
      | Abort =>
        (exists d1' r,
-          exec low o1 d1 abort (Finished d1' r) /\
-          o2 = [Cont] /\
-          d1' = (Some [], snd d1)) \/
+          exec imp u o1 d1 abort (Finished d1' r) /\
+          o2 = Cont /\
+          d1' = ([], snd d1)) \/
        
        (exists d1',
-          exec low o1 d1 abort (Crashed d1') /\
-          ((o2 = [CrashBefore] /\
-           d1' = d1) \/
-           (o2 = [CrashAfter] /\
-          d1' = (Some [], snd d1))))
+          exec imp u o1 d1 abort (Crashed d1') /\
+          o2 = CrashBefore /\
+          d1' = d1)
+
+      | Recover =>
+       (exists d1' r,
+          exec imp u o1 d1 recover (Finished d1' r) /\
+          o2 = Cont /\
+          d1' = d1) \/
+       
+       (exists d1',
+          exec imp u o1 d1 recover (Crashed d1') /\
+          o2 = CrashBefore /\
+          d1' = d1)
      end.
 
-   Definition refines_to (d1: state low) (d2: state high) :=     
-     exists l,
-       fst d1 = Some l /\
-       let txn_cache := apply_list empty_mem (rev l) in
-       fst d2 = txn_cache /\
-       addrs_match txn_cache (snd d1) /\
-       snd d2 = snd d1 /\
-       (forall a, a < data_length -> snd d1 a <> None).
+   Definition refines_to (d1: state imp) (d2: state abs) :=     
+     transaction_rep d1 d2.
+
+   Lemma exec_compiled_preserves_refinement_finished_core:
+    forall T (p2: abs_op.(Core.operation) T) o1 s1 s1' r u,
+        (exists s2, refines_to s1 s2) ->
+        imp.(exec) u o1 s1 (compile T p2) (Finished s1' r)->
+        (exists s2', refines_to s1' s2').
+  Proof. Admitted. (*
+    intros; destruct p2; simpl in *; cleanup.
+    {
+      eapply read_finished in H0; eauto; cleanup; eauto.
+    }
+    {
+      unfold refines_to in *; cleanup.
+      eapply write_finished in H0; eauto.
+      split_ors; cleanup; eauto.
+    }
+    {
+      unfold refines_to, cached_log_rep in *; cleanup.
+      eapply recover_finished in H0; eauto.
+      unfold cached_log_reboot_rep;
+      eexists; intuition eauto.      
+      eapply log_rep_to_reboot_rep_same; eauto.
+    }
+  Qed.
+   *)
 
    
-  Definition TransactionalDiskOperationRefinement := Build_OperationRefinement compile refines_to oracle_refines_to.
-  Definition TransactionalDiskRefinement := LiftRefinement high TransactionalDiskOperationRefinement.
+  Definition TransactionalDiskCoreRefinement := Build_CoreRefinement compile refines_to token_refines_to exec_compiled_preserves_refinement_finished_core.
+  Definition TransactionalDiskRefinement := LiftRefinement abs TransactionalDiskCoreRefinement.
+  
+  Notation "| p |" := (Op abs_op p)(at level 60).
+  Notation "x <-| p1 ; p2" := (Bind (Op abs_op p1) (fun x => p2))(right associativity, at level 60).
