src/Layers/BasicLayers/List/ListLayer.v
@@ -1,0 +1,64 @@
+Require Import Framework.
+Import ListNotations.
+
+Set Implicit Arguments.
+
+Section ListLayer.
+  
+  Variable V : Type.
+  
+  Inductive token' :=
+  | Crash : token'
+  | Cont : token'.
+
+  Definition state' := list V.
+  
+  Inductive list_prog : Type -> Type :=
+  | Get : list_prog (list V)
+  | Put : V -> list_prog unit
+  | Delete : list_prog unit.
+
+  
+  Inductive exec' :
+    forall T, user -> token' ->  state' -> list_prog T -> @Result state' T -> Prop :=
+  | ExecGet : 
+      forall d u,
+        exec' u Cont d Get (Finished d d)
+             
+  | ExecPut :
+      forall d v u,
+        exec' u Cont d (Put v) (Finished (v::d) tt)
+
+  | ExecDelete :
+      forall d u,
+        exec' u Cont d Delete (Finished [] tt)
+              
+  | ExecCrash :
+      forall T d (p: list_prog T) u,
+        exec' u Crash d p (Crashed d).
+
+  Hint Constructors exec' : core.
+  
+  Theorem exec_deterministic_wrt_token' :
+    forall u o s T (p: list_prog T) ret1 ret2,
+      exec' u o s p ret1 ->
+      exec' u o s p ret2 ->
+      ret1 = ret2.
+  Proof.
+    intros; destruct p; simpl in *; cleanup;
+    repeat
+      match goal with
+      | [H: exec' _ _ _ _ _ |- _] =>
+        inversion H; clear H; cleanup
+      end; eauto.
+  Qed.
+  
+  Definition ListOperation :=
+    Build_Core
+      list_prog
+      exec'
+      exec_deterministic_wrt_token'.
+
+  Definition ListLang := Build_Language ListOperation.
+  
+End ListLayer.
