src/Layers/ComposedLayers/TransactionCache/TransactionCacheLayer.v
@@ -1,13 +1,13 @@
-Require Import Framework.
-Require Export LoggedDiskLayer StorageLayer.
+Require Import Framework FSParameters.
+Require Export LoggedDiskLayer ListLayer.
 Import ListNotations.
 
 Set Implicit Arguments.
 
-Definition TransactionCacheOperation :=  HorizontalComposition (StorageOperation (list (addr * value))) LoggedDiskOperation.
+Definition TransactionCacheOperation :=  HorizontalComposition (ListOperation (addr * value)) (LoggedDiskOperation log_length data_length).
 Definition TransactionCacheLang := Build_Language TransactionCacheOperation.
 
-Notation "'|TCCP|' p" := (@lift_L1 (StorageOperation (list (addr * value))) LoggedDiskOperation (StorageLang (list (addr * value))) _ p) (at level 59).
-Notation "'|TCDP|' p" := (@lift_L2 (StorageOperation (list (addr * value))) LoggedDiskOperation LoggedDiskLang _ p) (at level 59).
-Notation "'|TCCO|' p" := (@lift_L1 (StorageOperation (list (addr * value))) LoggedDiskOperation (StorageLang (list (addr * value))) _ (Op (StorageOperation (list (addr * value))) p)) (at level 59).
-Notation "'|TCDO|' p" := (@lift_L2 (StorageOperation (list (addr * value))) LoggedDiskOperation LoggedDiskLang _ (Op LoggedDiskOperation p)) (at level 59).
+Notation "'|TCCP|' p" := (@lift_L1 (ListOperation (addr * value)) (LoggedDiskOperation log_length data_length) (ListLang (addr * value)) _ p) (at level 59).
+Notation "'|TCDP|' p" := (@lift_L2 (ListOperation (addr * value)) (LoggedDiskOperation log_length data_length) (LoggedDiskLang log_length data_length) _ p) (at level 59).
+Notation "'|TCCO|' p" := (@lift_L1 (ListOperation (addr * value)) (LoggedDiskOperation log_length data_length) (ListLang (addr * value)) _ (Op (ListOperation (addr * value)) p)) (at level 59).
+Notation "'|TCDO|' p" := (@lift_L2 (ListOperation (addr * value)) (LoggedDiskOperation log_length data_length) (LoggedDiskLang log_length data_length) _ (Op (LoggedDiskOperation log_length data_length) p)) (at level 59).
